joins.v
@@ -1,0 +1,381 @@
+Require Import List ListSet CpdtTactics basic fmaplist.
+
+Generalizable All Variables.
+Set Implicit Arguments.
+
+Definition in_list_list {A B} (l : list (A * (list B))) (a : A) (b : B) : Prop :=
+  exists bs, (MapsTo l a bs) /\ (set_In b bs).
+
+Section ListJoin.
+Variables (A B C : Type) (eq_dec : dec_type A)
+          (combine : list (A * B) -> B -> C -> B)
+          (base : list (A * B) -> C -> B).
+Fixpoint list_join  (l_orig : list (A * B))
+         (a : A) (c : C)
+         (l : list (A * B)) : list (A * B) :=
+  match l with
+      | nil => (a,base l_orig c)::nil
+      | (a',b)::l' => if (eq_dec a a') then
+                        (a,(combine l_orig b c))::l'
+                      else (a',b)::(list_join l_orig a c l')
+  end.
+Definition singleton {A} (eq_dec : dec_type A) (x : A) : list A := set_add eq_dec x (empty_set _).
+End ListJoin.
+
+Definition Subset {A} (s s' : set A) := forall x, In x s -> In x s'.
+Lemma subset_refl : forall A (s : set A), Subset s s.
+Proof. intros A s x Hin; auto. Qed.
+
+Lemma subset_trans : forall A (s s' s'' : set A) (Hsub0 : Subset s s') (Hsub1 : Subset s' s''), Subset s s''.
+Proof. intros; intros x Hin; apply Hsub0,Hsub1 in Hin; assumption. Qed.
+
+Inductive EntryLE {A B} (s : list (A * set B)) : A -> set B -> Prop :=
+  entryle_intro : forall a vs vs' (Hmap : MapsTo s a vs') (Hsub : Subset vs vs'), EntryLE s a vs.
+Definition MappingLE {A B} (s s' : list (A * set B)) := forall a vs (Hmap : MapsTo s a vs), EntryLE s' a vs.
+
+Section ListJoin_facts.
+Variables (A C : Type) (eq_dec : dec_type A)
+          (combine : list (A * list C) -> list C -> C -> list C)
+          (base : list (A * list C) -> C -> list C)
+          (Hextensive : (forall l b c, In c (combine l b c)))
+          (Hsingleton : (forall l c, In c (base l c))).
+Lemma in_list_join :
+  forall l l' a c,
+    (forall ab, In ab l -> In ab l') ->
+  in_list_list (list_join eq_dec combine base l' a c l) a c.
+Proof.
+  intros l l' a c Hcontain;
+  induction l as [|(a',b) l_ IH]; simpl;[
+  exists (base l' c); split; [left|]; apply Hsingleton; auto
+  |destruct (eq_dec a a') as [Heq | Hneq];
+   [subst; exists (combine l' b c); split; [left|apply Hextensive]
+   |assert (IHneed : (forall ab, In ab l_ -> In ab l')) by (intros (a_,bs') Hin; apply Hcontain; right; auto);
+     set (mumble := (IH IHneed));
+     inversion mumble as [wit Hwit]; subst; destruct Hwit as [Hmap Hin];
+     exists wit; split; [apply map_rst|]]; auto].
+Qed.
+
+Lemma unmapped_join : `{Unmapped l a -> a <> a' -> Unmapped (list_join eq_dec combine base l' a' c l) a}.
+Proof.
+  induction l as [|(a,b) l_ IH]; intros a0 a' l' c H ?;
+   simpl; [repeat constructor
+          |destruct (eq_dec a' a) as [Heq|Hneq];
+            [subst; inversion H; constructor
+            |constructor;inversion H;[apply IH|]]]; auto.
+Qed.
+
+Lemma functional_join : `{Functional l -> Functional (list_join eq_dec combine base l' a c l)}.
+Proof.
+  induction l as [|(a,b) l_ IH]; simpl;
+  [intros; repeat constructor
+  |intros l' a' c F].
+  destruct (eq_dec a' a) as [Heq|Hneq];
+  [subst; apply functional_exchange with (b := b)
+  |constructor; inversion F; [apply IH|apply unmapped_join]]; auto.
+Qed.
+
+
+Lemma maple_refl : forall (l : list (A * set C)), MappingLE l l.
+Proof. 
+  induction l as [|(a_,b_) l_ IH]; intros a' b' Hmap;
+  [inversion Hmap
+  |apply entryle_intro with (vs' := b'); [|apply subset_refl]; auto].
+Qed.
+
+Lemma maple_trans: forall (l l' l'' : list (A * set C)) (Hmap0 : MappingLE l l') (Hmap1 : MappingLE l' l''), MappingLE l l''.
+Proof.
+  intros; intros a cs Hmap;
+  pose (mumble := Hmap0 a cs Hmap);
+  inversion mumble as [? ? cs' map' sub']; subst;
+  pose (grumble := Hmap1 a cs' map');
+  inversion grumble as [? ? cs'' map'' sub'']; subst;
+  exists cs'';[|apply subset_trans with (s' := cs')]; auto.
+Qed.
+
+Lemma maple_top : forall (l : list (A * set C)) a b b', Subset b b' -> MappingLE ((a,b) :: l) ((a,b') :: l).
+Proof.
+  intros.
+  intros a' b'' Hmap.
+  inversion Hmap as [|? ? ? ? ? Hneq Hmap']; subst.
+  apply entryle_intro with (vs' := b');[constructor|assumption].
+  apply entryle_intro with (vs' := b'');[constructor; auto|apply subset_refl].
+Qed.
+
+Lemma maple_bottom : forall (l l' : list (A * set C)) ab (Htail : MappingLE l l'), MappingLE (ab :: l) (ab :: l').
+Proof.
+  intros. 
+  intros ? ? Hmap; inversion Hmap as [|? ? ? ? ? Hneq Hmap']; subst;
+  [exists vs; [constructor|apply subset_refl]
+        |].
+  pose (mumble := Htail a vs Hmap').
+  inversion mumble as [? ? vs' Hmap_ Hsub_]; subst.
+  exists vs'; [constructor|]; auto.
+Qed.
+
+Variable Hextensive' : (forall l b c c', In c' b -> In c' (combine l b c)).
+Lemma in_list_join2 :
+  forall l l' a a' c c',
+  in_list_list l a' c' ->
+  in_list_list (list_join eq_dec combine base l' a c l) a' c'.
+Proof.
+  intros l l' a a' c c' Hold;
+  induction l; simpl;
+  inversion Hold as [bs Hwit]; destruct Hwit as [Hpairin Hsetin]; subst;
+  [(* base case *) inversion Hpairin
+  |destruct a0; destruct (eq_dec a a0) as [Heq | Hneq]; subst;
+   [(* Heq *)
+     subst; inversion Hpairin; subst;
+    [exists (combine l' bs c); split; [left|apply Hextensive']; auto
+           |exists bs; split; [right|]; auto]
+   |(* Hneq *)
+    destruct (eq_dec a0 a') as [Heq' | Hneq'];
+     inversion Hpairin as [|? ? ? ? ? ? Hmap']; subst;
+    [exists bs; split; [constructor|]; auto
+    |bad_eq
+    |exists bs; constructor; [constructor|]; auto
+    |assert (IHneed : in_list_list l a' c') by (exists bs; repeat constructor; auto);
+     set (IHl_ := IHl IHneed);
+     inversion IHl_ as [x Hwit]; destruct Hwit as [Hmap Hin];
+     exists x; repeat constructor; auto]]].
+Qed.
+
+Lemma non_join_untouched : forall l l' a a' c b
+                             (Hneq : a <> a')
+                             (H: MapsTo (list_join eq_dec combine base l' a c l) a' b),
+                             MapsTo l a' b.
+Proof.
+  induction l as [|(a_,b_) l_ IH]; intros;
+  [inversion H; subst; [contradict Hneq|]; auto
+  |
+  simpl in H; inversion H as [? ? rst H'|? a'' ? ? ? Hneq'' map' Hinj]; subst;
+  destruct (eq_dec a a_) as [Heq_|Hneq_];
+  try (injection H'; intros; subst);
+  try (injection Hinj; intros; subst);
+  [
+  (* Eq *)
+  constructor; [auto
+               |apply IH with (l' := l') (a := a_) (c := c);
+                 [auto
+                 |contradict Hneq; auto]]
+  |constructor
+  |subst; constructor; auto
+  |constructor; [auto | apply IH with (l' := l') (a := a) (c := c); auto]]].
+Qed.
+
+(*
+  
+Lemma unmapped_join2 : forall l a a' b c l'
+                             (Hcontain : (forall a c, in_list_list l a c -> in_list_list l' a c)
+                                          \/ (b = (base l' c))),
+                        Unmapped l a' ->
+                        MapsTo (list_join eq_dec combine base l' a c l) a' b ->
+                        (b = (base l' c)) /\ a = a'.
+Proof.
+  induction l as [|(a_,b_) l_ IH];
+  simpl; intros a a' b c l' Hcontain Hunmap Hmap;
+  [inversion Hmap as [|? ? ? ? ? ? Hbad]; subst; split; solve [auto|reflexivity|inversion Hbad]
+  |].
+  destruct (eq_dec a a_) as [Heq | Hneq];
+    [inversion Hunmap as [|? ? ? ? Hunmap' Hneq]; subst;
+     inversion Hmap as [|? ? ? ? ? ? Hbad]; split; try solve [reflexivity|
+                                             rewrite unmapped_not_mapped in Hunmap';
+                                             [apply Hunmap' in Hbad; contradiction
+                                             |auto]]
+    |].
+  inversion Hmap as [|? ? ? ? ? ? Hbad]; subst; contradict Hneq; auto.
+  apply IH with (b := b) (c := c) (l' := l').
+  inversion Hcontain as [L|R].
+  specialize L with a_ b_
+  intros a_' c_' Hin; inversion Hin as [bs_ [Hmap_ Hsetin_]];
+  apply Hcontain; destruct (eq_dec a_' a_) as [Heq_|Hneq_];
+  [subst
+    |exists bs_; repeat constructor]; auto.
+  unfold in_list_list.
+  Focus 2.
+  
+    [intros a_' c_' Hin
+    |inversion Hunmap
+    |]; auto.
+
+; 
+  inversion Hmap; [(* a_' = a_ *)
+                   rewrite unmapped_not_mapped in Hunmap; [
+                    (* rewritten *)
+                    subst; match goal with [bad : ?a <> ?a |- _] => contradict bad; auto end
+                    |(* satisfy hyp *)assumption]
+                   |subst]. 
+  Check unmapped_not_mapped.
+                       
+   [specialize Hunmap with b; contradict Hunmap; constructor
+   |assumption
+   |
+   |assumption].
+  .
+  ; constructor; auto | auto].
+    
+
+ subst; repeat constructor|]
+  constructor.
+Qed.
+Admitted.*)
+
+End ListJoin_facts.
+Section ListJoin_morefacts.
+Variables (A C : Type) (eq_dec : dec_type A) (ceq_dec : dec_type C).
+Definition joiner := (fun (_ : list (A * list C)) κs κ => (set_add ceq_dec κ κs)).
+Definition singler := (fun (_ : list (A * list C)) c => (singleton ceq_dec c)).
+Hint Unfold singleton singler.
+
+(* set_In cc (joiner ll' cs cc) *)
+Lemma In_same : forall l cs c (H : set_In c cs), (joiner l cs c) = cs.
+Proof.
+  induction cs; intros; simpl in H;[contradiction|inversion H as [L|R]];
+  simpl; destruct (ceq_dec c a) as [Heq|Hneq];
+  try solve [auto | contradict Hneq; auto | f_equal; apply IHcs; auto].
+Qed.
+
+Lemma In_neq : forall c c' l cs (Hin : set_In c' (joiner l cs c)) (Hneq : c <> c'), set_In c' cs.
+Proof.
+  induction cs as [|c_ l_ IH]; simpl; intros; [inversion Hin; auto|].
+  destruct (ceq_dec c c_) as [Heq|Hneq_].
+  inversion Hin; [left|right]; auto.
+  inversion Hin; [left|]; auto.
+Qed.
+
+Lemma set_add_elim2 : forall a b ignore (l : set C) (H : set_In a (joiner ignore l b)),
+                        (a = b /\ ~ set_In b l) \/ (set_In a l).
+Proof.
+  induction l; simpl; [intuition|].
+  destruct (ceq_dec b a0) as [Heq|Hneq].
+  (* eq *)
+  subst; intros H';
+  inversion H'; subst.
+  destruct IHl as [[? Bad]|]; [apply set_add_intro2; auto|intuition|intuition].
+  intuition.
+  (* neq *)
+  intros H'; inversion H'; subst; [intuition|].
+  destruct IHl as [[? Bad]|]; intuition.
+Qed.
+
+Lemma in_list_join_set_split : forall (l l' : list (A * list C))
+                                      (a a' : A)
+                                      (c c' : C)
+                                 (Hin : in_list_list (list_join eq_dec joiner singler l' a c l) a' c'),
+                                 ((a = a') /\ (c = c') /\ (~ in_list_list l a c)) \/ (in_list_list l a' c').
+Proof.
+  induction l as [|(a,cs) l_ IH]; [intros|intros ll' aa aa' cc cc' Hin];
+  simpl in *; 
+  inversion Hin as [cs_ Hwit]; destruct Hwit as [map_ in_]; subst.
+  (* base case *)
+  inversion map_ as [bad0 bad1 bad2 bad3 bad4 bad5|bad0 bad1 bad2 bad3 bad4 bad5 bad6]; subst;
+  [inversion in_ as [bad0|bad]; [subst; left; repeat split; intro bad;
+                                 inversion bad as [bbad0 [bbad1 ?]]; auto; inversion bbad1
+                                |inversion bad]
+  |inversion bad6].
+
+  destruct (eq_dec aa a) as [Heq|Hneq];
+    inversion map_ as [|foo bar baz qux moo boo too];subst.
+  subst.
+  (* Eq case with inversion *)
+
+  destruct (set_add_elim2 _ _ _ _ in_) as [Hceq|Hinrest];
+       [destruct Hceq as [H H0]
+       |subst; right; exists cs; repeat constructor; auto].
+  
+  left; repeat split; auto; intros [X [HH0 HH1]];
+  assert (damn : X = cs) by
+      (inversion HH0; subst; [|match goal with [bad : ?a <> ?a |- _] => contradict bad; auto end]; auto);
+  subst; apply H0; auto.
+
+  right; destruct Hin as [bad [Hbad0 Hbad1]];
+  inversion Hbad0; subst; [contradict boo|]; auto;
+  exists bad; split; [constructor|]; auto.
+
+  right; exists cs_; split; [constructor|]; auto.
+  destruct IH with (l' := ll') (a := aa) (a' := aa') (c := cc) (c' := cc') as [[? [? ?]]|[X [? ?]]];
+    [exists cs_; split; auto
+    |left; repeat split; auto; intro bad; inversion bad as [X [mum ble]]; inversion mum; subst; [bad_eq|apply H1; exists X; split; auto]
+    |right; exists X; split; [constructor|]; auto].
+Qed.
+
+End ListJoin_morefacts.
+
+Inductive Dom_in_Dom {A B C} : list (A * B) -> list (A * C) -> Prop :=
+  | no_dom : `{Dom_in_Dom nil l}
+  | cons_dom : `{InDom l' a -> Dom_in_Dom l l' -> Dom_in_Dom ((a,b)::l) l'}.
+Hint Constructors Dom_in_Dom.
+
+Lemma list_join_ordering : forall (A B C : Type) (eq_dec : dec_type A)
+                                  (combine : list (A * list B) -> list B -> C -> list B)
+                                  (base : list (A * list B) -> C -> list B)
+                                  (Hextensive' : (forall l b c c', In c' b -> In c' (combine l b c)))
+                                  l l' a c,
+                             MappingLE l (list_join eq_dec combine base l' a c l).
+Proof.
+  induction l as [|(a_,b_) l_ IH]; intros;
+  [intros ? ? bad; inversion bad
+  |simpl; destruct (eq_dec a a_) as [Heq|Hneq];
+   [subst; apply maple_top; intros ? ?; apply Hextensive'; auto
+   |apply maple_bottom, IH]].
+Qed.
+
+Lemma Dom_InDom : forall A B C (eq_dec : dec_type A) (l : list (A * B)) (l' : list (A * C)) (Hdom : Dom_in_Dom l l')
+                         a
+                         (Hindom : InDom l a), InDom l' a.
+Proof.
+induction l; intros; [inversion Hindom|inverts Hdom;destruct (eq_dec a1 a0) as [Heq|Hneq]; [subst; auto|inversion Hindom; [subst; contradict Hneq|apply IHl]; auto]].
+Qed.
+
+Lemma In_join : forall A B C (eq_dec : dec_type A) (l l' : list (A * B))
+                        (f : list (A * B) -> B -> C -> B)  g a a' b b'
+                        (Hcontain : (forall a b, In (a,b) l -> In (a,b) l'))
+                        (H : In (a,b) l),
+                  (exists b'', In (a,b'') (list_join eq_dec f g l' a' b' l)).
+Proof.
+  intros A B C eq_dec l l' f g a a' b b' Hcontain Hin; induction l as [|(a0,b0) l_ IH];
+  inverts Hin;
+  assert (IHneed : forall a b, In (a,b) l_ -> In (a,b) l') by
+      (intros; apply Hcontain; right; auto);
+  pose (rec := IH IHneed);
+  [injection H; intros; subst;
+   unfold list_join;
+   destruct (eq_dec a' a) as [Heq | Hneq];[
+     subst; exists (f l' b b')
+   |exists b]; constructor; auto
+  |unfold list_join;
+    destruct (eq_dec a' a0) as [Heq | Hneq];[
+      exists b; right; auto
+           |destruct rec as [b'' Hb'']; auto; exists b''; right; auto]].
+Qed.
+
+Lemma Dom_join_right : forall A B C D (eq_dec : dec_type A) (l : list (A * B)) (l' : list (A * D))
+                        (f : list (A * D) -> D -> C -> D)  g a b,
+                   Dom_in_Dom l l' -> Dom_in_Dom l (list_join eq_dec f g l' a b l').
+Proof.
+  intros A B C D eq_dec l l' f g a b Hdom; induction Hdom as [|? ? ? ? H];
+  constructor;
+  (induction l';[rewrite InDom_In in H; auto; destruct H as [? bad]; inversion bad |]);
+  [rewrite InDom_In in H; auto; destruct H as [b' Hb'];
+   rewrite InDom_In; auto; apply In_join with (b := b')|]; auto.
+Qed.
+
+Lemma Dom_join_left : forall A B C D (eq_dec: dec_type A) (l l_ : list (A * B)) (l' : list (A * D))
+                        (f : list (A * B) -> B -> C -> B)  g a b
+                        (Hcontain: (forall ab, In ab l -> In ab l_)),
+                   Dom_in_Dom l l' ->
+                   (exists d, MapsTo l' a d) ->
+                   Dom_in_Dom (list_join eq_dec f g l_ a b l) l'.
+Proof.
+  intros A B C D eq_dec l l_ l' f g a b Hcontain Hdom [d Hin]; induction Hdom.
+  (* base *)
+  repeat constructor; rewrite InDom_is_mapped; auto; exists d; auto.
+    (* induction step *)
+  simpl; destruct (eq_dec a a0) as [Heq|Hneq]; subst; simpl;
+  [constructor; [rewrite InDom_is_mapped; auto; exists d|]; auto
+  |].
+  rewrite InDom_In in H; auto; destruct H as [d' Hin'].
+  constructor;
+    [rewrite InDom_In; auto; exists d'
+    |apply IHHdom; [intros; apply Hcontain; right|]]; auto.
+Qed.
+
